Guess adequate memory relation for inlining (extension of Mem.inject).

common/MemoryRelation.v
@@ -43,7 +43,7 @@ Record mrelT: Type := mkmrelT {
 Definition mrelT_ops_equals: mrelT_opsT unit :=
   mkmrelT_opsT
     (fun _ m1 m2 => m1 = m2)
-    (fun _ v1 v2 => Val.lessdef v1 v2)
+    (fun _ v1 v2 => v1 = v2)
     (fun _ _ => True)
     (fun _ _ => True)
     (fun _ _ _ _ _ => tt).
@@ -51,7 +51,15 @@ Definition mrelT_ops_equals: mrelT_opsT unit :=
 Program Definition mrelT_props_equals: mrelT_propsT mrelT_ops_equals := mkmrelT_propsT _ _ _ _ _ _.
 Next Obligation. repeat constructor. Qed.
 Next Obligation. repeat constructor. Qed.
-Next Obligation. inv H. auto. Qed.
+
+Lemma mrelT_ops_equals_list_equal mrel v1 v2:
+  v1 = v2 <-> list_forall2 (mrelT_ops_equals.(sem_value) mrel) v1 v2.
+Proof.
+  revert v2.
+  induction v1; intros; constructor; intro H; inv H; simpl; try constructor; auto.
+  - apply IHv1. auto.
+  - inv H2. f_equal. apply IHv1. auto.
+Qed.
 
 (* extends *)
 
@@ -79,22 +87,69 @@ Proof.
 Qed.
 
 (* inject *)
-Definition mrelT_ops_inject: mrelT_opsT meminj :=
+Structure mrelT_inject: Type := mkmrelT_inject {
+  mrelT_meminj: meminj;
+  mrelT_src: mem;
+  mrelT_tgt: mem
+}.
+
+Inductive mrelT_sem (mrel:mrelT_inject) (m_src m_tgt:mem): Prop :=
+| mrelT_sem_intro
+    (Hinject: Mem.inject mrel.(mrelT_meminj) m_src m_tgt)
+    (Hsrc: mrel.(mrelT_src) = m_src)
+    (Htgt: mrel.(mrelT_tgt) = m_tgt)
+.
+
+Inductive mrelT_le (mrel1 mrel2:mrelT_inject): Prop :=
+| mrelT_le_intro
+    (INCR: inject_incr mrel1.(mrelT_meminj) mrel2.(mrelT_meminj))
+    (LE: Ple (Mem.nextblock mrel1.(mrelT_tgt)) (Mem.nextblock mrel2.(mrelT_tgt)))
+    (INJ: forall b1 b2 delta, 
+          mrel2.(mrelT_meminj) b1 = Some(b2, delta) -> Plt b2 (Mem.nextblock mrel1.(mrelT_tgt)) -> mrel1.(mrelT_meminj) b1 = Some(b2, delta))
+    (PERM1: forall b1 b2 delta ofs,
+          mrel2.(mrelT_meminj) b1 = Some(b2, delta) -> Plt b2 (Mem.nextblock mrel1.(mrelT_tgt)) ->
+          Mem.perm mrel2.(mrelT_src) b1 ofs Max Nonempty -> Mem.perm mrel1.(mrelT_src) b1 ofs Max Nonempty)
+    (PERM2: forall b ofs, Plt b (Mem.nextblock mrel1.(mrelT_tgt)) ->
+          Mem.perm mrel1.(mrelT_tgt) b ofs Cur Freeable -> Mem.perm mrel2.(mrelT_tgt) b ofs Cur Freeable)
+    (PERM3: forall b ofs k p, Plt b (Mem.nextblock mrel1.(mrelT_tgt)) ->
+          Mem.perm mrel2.(mrelT_tgt) b ofs k p -> Mem.perm mrel1.(mrelT_tgt) b ofs k p)
+.
+
+Program Instance PreOrder_mrelT_le: PreOrder mrelT_le.
+Next Obligation. constructor; intros; auto. reflexivity. Qed.
+Next Obligation.
+  repeat intro. inv H. inv H0. constructor; intros; auto.
+  - eapply inject_incr_trans; eauto.
+  - rewrite LE. auto.
+  - eapply INJ; eauto. eapply INJ0; eauto.
+    eapply Plt_Ple_trans; eauto.
+  - eapply PERM1; eauto. eapply INJ0; eauto.
+    eapply Plt_Ple_trans; eauto.
+    eapply PERM0; eauto.
+    eapply Plt_Ple_trans; eauto.
+  - eapply PERM4; eauto.
+    eapply Plt_Ple_trans; eauto.
+  - eapply PERM3; eauto. eapply PERM5; eauto.
+    eapply Plt_Ple_trans; eauto.
+Qed.
+
+Definition mrelT_ops_inject: mrelT_opsT mrelT_inject :=
   mkmrelT_opsT
-    Mem.inject
-    val_inject
-    inject_incr
-    inject_incr
-    (fun _ _ _ m _ => Mem.flat_inj (Mem.nextblock m)).
+    mrelT_sem
+    (fun mrel => val_inject mrel.(mrelT_meminj))
+    mrelT_le
+    mrelT_le
+    (fun _ _ _ m _ => mkmrelT_inject (Mem.flat_inj (Mem.nextblock m)) m m).
 
 Program Definition mrelT_props_inject: mrelT_propsT mrelT_ops_inject := mkmrelT_propsT _ _ _ _ _ _.
-Next Obligation. constructor; repeat intro; auto. Qed.
-Next Obligation. constructor; repeat intro; auto. Qed.
 Next Obligation. inv H. auto. Qed.
-Next Obligation. eapply Genv.initmem_inject; eauto. Qed.
+Next Obligation.
+  constructor; auto. simpl.
+  eapply Genv.initmem_inject; eauto.
+Qed.
 
 Lemma mrelT_ops_inject_list_inject mrel v1 v2:
-  val_list_inject mrel v1 v2 <-> list_forall2 (mrelT_ops_inject.(sem_value) mrel) v1 v2.
+  val_list_inject mrel.(mrelT_meminj) v1 v2 <-> list_forall2 (mrelT_ops_inject.(sem_value) mrel) v1 v2.
 Proof.
   revert v2.
   induction v1; intros; constructor; intro H; inv H; constructor; auto.
